src/Funtab.v
@@ -1,0 +1,48 @@
+(** Funtab.
+  This file defines the [Funtab] type, used to store built-in R functions.
+  The function names of this file correspond to the function names
+  in the file include/Defn.h. **)
+
+(* Copyright © 2022 Martin Bodin
+
+  This program is free software; you can redistribute it and/or modify
+  it under the terms of the GNU General Public License as published by
+  the Free Software Foundation; either version 2 of the License, or
+  (at your option) any later version.
+
+  This program is distributed in the hope that it will be useful,
+  but WITHOUT ANY WARRANTY; without even the implied warranty of
+  MERCHANTABILITY or FITNESS FOR A PARTICULAR PURPOSE.  See the
+  GNU General Public License for more details.
+
+  You should have received a copy of the GNU General Public License
+  along with this program; if not, write to the Free Software
+  Foundation, Inc., 51 Franklin St, Fifth Floor, Boston, MA  02110-1301 USA *)
+
+Set Implicit Arguments.
+From CoqR Require Import Result.
+
+(** The [Funtab] effect in Result calls a function with the following type. **)
+Definition funtab_function :=
+  SEXP -> (** call **)
+  SEXP -> (** op **)
+  SEXP -> (** args **)
+  SEXP -> (** rho **)
+  mRHFJE SEXP.
+
+(** The [FUNTAB] is then an array of such functions, with some
+  additional meta-data, like the function name: **)
+Record funtab_cell := make_funtab_cell {
+    fun_name : string ;
+    fun_cfun : funtab_function ;
+    fun_code : int ; (** The number stored here can be quite large. We thus use [int] instead of [nat]. **)
+    fun_eval : funtab_eval_arg ;
+    fun_arity : int ;
+    fun_gram : PPinfo
+  }.
+
+Instance funtab_cell_Inhab : Inhab funtab_cell.
+Proof. apply Inhab_of_val. constructors; apply arbitrary. Defined.
+
+Definition funtab := ArrayList.array funtab_cell.
+
