src/Operators.v
@@ -1,0 +1,132 @@
+(** Result.
+  This file describes the [result] monad. **)
+
+(* Copyright © 2022 Martin Bodin
+
+  This program is free software; you can redistribute it and/or modify
+  it under the terms of the GNU General Public License as published by
+  the Free Software Foundation; either version 2 of the License, or
+  (at your option) any later version.
+
+  This program is distributed in the hope that it will be useful,
+  but WITHOUT ANY WARRANTY; without even the implied warranty of
+  MERCHANTABILITY or FITNESS FOR A PARTICULAR PURPOSE.  See the
+  GNU General Public License for more details.
+
+  You should have received a copy of the GNU General Public License
+  along with this program; if not, write to the Free Software
+  Foundation, Inc., 51 Franklin St, Fifth Floor, Boston, MA  02110-1301 USA *)
+
+From CoqR Require Import Result.
+From ITree Require Export ITree.
+
+Import EventMonad.
+Import ITree.Eq.Eqit.
+
+(** * Notations *)
+
+Declare Scope result_scope.
+
+Module ResultNotations.
+
+Delimit Scope result_scope with res.
+
+Notation "c >>= f" :=
+  (@EventMonad.bind _ _ _ _ c%res f%res)
+  (at level 58, left associativity) : result_scope.
+
+Notation "f =<< c" :=
+  (@EventMonad.bind _ _ _ _ c%res f%res)
+  (at level 61, right associativity) : result_scope.
+
+Notation "f >=> g" :=
+  (@rcompose _ _ _ _ _ f g)
+  (at level 61, right associativity) : result_scope.
+
+Notation "e1 ;; e2" :=
+  (@EventMonad.bind _ _ _ _ e1%res (fun _ => e2%res))
+  (at level 61, right associativity) : result_scope.
+
+Notation "'let*' p ':=' c1 'in' c2" :=
+  (@EventMonad.bind _ _ _ _ c1%res (fun p => c2%res))
+  (at level 61, p as pattern, c1 at next level, right associativity) : result_scope.
+  
+Notation "x <- c1 ;; c2" :=
+  (@EventMonad.bind _ _ _ _ c1%res (fun x => c2%res))
+  (at level 61, c1 at next level, right associativity) : result_scope.
+
+Notation "' pat <- c1 ;; c2" :=
+  (@EventMonad.bind _ _ _ _ c1%res (fun x => match x with pat => c2%res end))
+  (at level 61, pat pattern, c1 at next level, right associativity) : result_scope.
+
+Notation "` v" :=
+  (@EventMonad.ret _ v)
+  (at level 10, v at next level, no associativity) : result_scope.
+
+Notation "'return' v" :=
+  (@EventMonad.ret _ v)
+  (at level 10, v at next level, no associativity) : result_scope.
+
+End ResultNotations.
+
+Import ResultNotations.
+Open Scope result_scope.
+
+
+(** * Boolean Operations *)
+
+Definition mR_lift [A B] (op : A -> B)
+  d (b : result d A) : result d B :=
+  ltac:(simplify_term (
+    b <- b ;;
+    return (op b))).
+
+Lemma mR_lift2_value : forall A B C (op : A -> B -> C) a b,
+  (mR_lift2 op _ _ (`a) (`b))%res ≅ return (op a b).
+Proof. intros. tau_steps. reflexivity. Qed.
+
+Definition mR_lift2 [A B C] (op : A -> B -> C)
+    d1 d2 (b1 : result d1 A) (b2 : result d2 B) : result _ C :=
+  b1 <- b1 ;;
+  b2 <- b2 ;;
+  return (op b1 b2).
+
+Lemma mR_lift2_value : forall A B C (op : A -> B -> C) a b,
+  (mR_lift2 op _ _ (`a) (`b))%res ≅ return (op a b).
+Proof. intros. tau_steps. reflexivity. Qed.
+
+Section Booleans.
+
+Open Scope bool_scope.
+
+Set Printing All.
+
+Definition mR_and := mR_lift andb.
+
+Notation "a && b" := (mR_and _ _ a b) (at level 40, left associativity) : result_scope.
+
+Definition mR_or := mR_lift orb.
+
+Infix "'||" := mR_or (at level 50, left associativity) : result_scope.
+
+Notation "'! b" := (mR_neg b) (at level 35, right associativity).
+
+Lemma mR_neg_bool : forall b : bool,
+  '! b ≅ (negb b : mR_bool).
+Proof. intros. tau_steps. reflexivity. Qed.
+
+Definition mR_decide P `{Decidable P} : mR_bool := decide P.
+Arguments mR_decide P {_}.
+
+Notation "''decide' P" := (mR_decide P) (at level 70, no associativity).
+
+Definition mR_eq_SEXP : mR_SEXP -> mR_SEXP -> mR_bool := @mR_eq _ _.
+
+Infix "'==" := mR_eq (at level 70, no associativity).
+
+Notation "a '!= b" := ('! (a '== b)) (at level 70, no associativity).
+
+Notation "'ifc' b 'then' v1 'else' v2" :=
+  (x <- (b : mR_bool) ;; if x then v1 else v2)
+  (at level 200, right associativity) : type_scope.
+*)
